Refactor ann to Annotation.

AbsInt.v
@@ -1,7 +1,7 @@
 Require Import CSet Le.
 
 Require Import Plus Util AllInRel Map.
-Require Import Val Var Env EnvTy IL Lattice DecSolve LengthEq MoreList.
+Require Import Val Var Env EnvTy IL Annotation Lattice DecSolve LengthEq MoreList.
 
 Class AbstractInterpretation Dom FunDom `{SemiLattice Dom} := {
   transform : list FunDom -> stmt -> ann Dom -> Dom;                                  
@@ -11,27 +11,27 @@ Class AbstractInterpretation Dom FunDom `{SemiLattice Dom} := {
 Fixpoint backward {Dom} {FunDom} `{SemiLattice Dom} (AI:AbstractInterpretation Dom (FunDom)) 
          (st:stmt) (AL:list FunDom) (a:ann Dom) {struct st} : ann Dom :=
   match st, a with
-    | stmtExp x e s as st, annExp d ans => 
+    | stmtExp x e s as st, ann1 d ans => 
       let ans' := backward AI s AL ans in
-      let d' := annExp d ans' in
-      annExp (transform AL st d') ans'
-    | stmtIf x s t as st, annIf d ans ant =>
+      let d' := ann1 d ans' in
+      ann1 (transform AL st d') ans'
+    | stmtIf x s t as st, ann2 d ans ant =>
       let ans' := backward AI s AL ans in
       let ant' := backward AI t AL ant in
-      let an' := (annIf d ans' ant') in
-      annIf (transform AL st an') ans' ant'
+      let an' := (ann2 d ans' ant') in
+      ann2 (transform AL st an') ans' ant'
       
-    | stmtGoto f Y as st, annGoto d as an => 
-      annGoto (transform AL st an)
+    | stmtGoto f Y as st, ann0 d as an => 
+      ann0 (transform AL st an)
 
-    | stmtReturn x as st, annReturn d as an => 
-      annReturn (transform AL st an)
+    | stmtReturn x as st, ann0 d as an => 
+      ann0 (transform AL st an)
 
-    | stmtLet Z s t as st, annLet d ans ant => 
+    | stmtLet Z s t as st, ann2 d ans ant => 
       let ans' := backward AI s (mkFunDom Z ans::AL) ans in
       let ant' := backward AI t (mkFunDom Z ans'::AL) ant in
-      let d' := annLet d ans' ant' in
-      annLet (transform (mkFunDom Z ans'::AL)
+      let d' := ann2 d ans' ant' in
+      ann2 (transform (mkFunDom Z ans'::AL)
                         st 
                         d') ans' ant'
     | _, an => an
@@ -54,26 +54,18 @@ Defined.
 
 
 Inductive ann_lt {A} (R:A->A->Prop) : ann A -> ann A -> Prop :=
-  | annLtExp a b an bn 
+  | annLt1 a b an bn 
     : R a b 
       -> ann_lt R an bn 
-      -> ann_lt R (annExp a an) (annExp b bn)
-  | annLtIf a ans ant b bns bnt
+      -> ann_lt R (ann1 a an) (ann1 b bn)
+  | annLt2 a ans ant b bns bnt
     : R a b
       -> ann_lt R ans bns 
       -> ann_lt R ant bnt 
-      -> ann_lt R (annIf a ans ant) (annIf b bns bnt)
-  | annLtGoto a b
+      -> ann_lt R (ann2 a ans ant) (ann2 b bns bnt)
+  | annLt0 a b
       : R a b
-      -> ann_lt R (annGoto a) (annGoto b)
-  | annLtReturn a b
-      : R a b
-      -> ann_lt R (annReturn a) (annReturn b)
-  | annLtLet a ans ant b bns bnt
-    : R a b
-      -> ann_lt R ans bns 
-      -> ann_lt R ant bnt 
-      -> ann_lt R (annLet a ans ant) (annLet b bns bnt).
+      -> ann_lt R (ann0 a) (ann0 b).
 
 
 
@@ -109,14 +101,11 @@ Proof.
   constructor.
   revert a b.
   fix 1.
-  destruct a; destruct b; try now (right; intro; isabsurd).
-  + destruct_prop (R a a1); edestruct ann_lt_dec with (a:=a0) (b:=b); 
-    hnf in *; try eassumption; try dec_solve.
-  + destruct_prop (R a1 a); edestruct ann_lt_dec with (a:=a2) (b:=b1); 
-    edestruct ann_lt_dec with (a:=a3) (b:=b2); hnf in *; 
+  destruct a; destruct b; try dec_solve.
+  + destruct_prop (R a a0); dec_solve. 
+  + destruct_prop (R a a1); try dec_solve;
+    edestruct ann_lt_dec with (a:=a0) (b:=b); hnf in *; 
     try eassumption; try dec_solve. 
-  + destruct_prop (R a a0); hnf in *; try eassumption; try dec_solve.
-  + destruct_prop (R a a0); hnf in *; try eassumption; try dec_solve. 
   + destruct_prop (R a1 a); try dec_solve.
     destruct (ann_lt_dec a2 b1); try dec_solve.
     destruct (ann_lt_dec a3 b2); try dec_solve.
