IL/Annotation.v
@@ -1,0 +1,87 @@
+Require Import List.
+Require Export Util Relations Get Drop Var Val Exp Env Map CSet AutoIndTac MoreList IL.
+
+Set Implicit Arguments.
+
+Inductive ann (A:Type) : Type :=
+| ann0 (a:A) : ann A
+| ann1 (a:A) (sa:ann A) : ann A
+| ann2 (a:A) (sa:ann A) (ta:ann A) : ann A.
+ 
+Definition getAnn {A} (a:ann A) : A :=
+match a with
+| ann0 a => a
+| ann1 a _ => a
+| ann2 a _ _ => a
+end.
+
+Fixpoint setAnn A (s:stmt) (a:A) : ann A :=
+  match s with
+   | stmtExp x e s' => ann1 a (setAnn s' a)
+   | stmtIf x s1 s2 => ann2 a (setAnn s1 a) (setAnn s2 a)
+   | stmtGoto l Y => ann0 a
+   | stmtReturn x => ann0 a
+   | stmtLet Z s1 s2 => ann2 a (setAnn s1 a) (setAnn s2 a)
+   end.
+
+Fixpoint setTopAnn A (s:ann A) (a:A) : ann A :=
+  match s with
+   | ann0 _ => ann0 a
+   | ann1 _ s' => ann1 a s'
+   | ann2 _ s1 s2 => ann2 a s1 s2
+   end.
+
+Fixpoint mapAnn X Y (f:X->Y) (a:ann X) : ann Y := 
+  match a with
+    | ann1 a an => ann1 (f a) (mapAnn f an)
+    | ann2 a an1 an2 => ann2 (f a) (mapAnn f an1) (mapAnn f an2) 
+    | ann0 a => ann0 (f a)
+  end.
+
+Lemma getAnn_mapAnn A A' (a:ann A) (f:A->A')
+  : getAnn (mapAnn f a) = f (getAnn a).
+Proof.
+  general induction a; simpl; eauto.
+Qed.
+
+Inductive annotation {A:Type} : stmt -> ann A -> Prop :=
+| antExp x e s a sa 
+  : annotation s sa 
+    -> annotation (stmtExp x e s) (ann1 a sa)
+| antIf x s t a sa ta 
+  : annotation s sa 
+    -> annotation t ta 
+    -> annotation (stmtIf x s t) (ann2 a sa ta)
+| antGoto l Y a 
+  : annotation (stmtGoto l Y) (ann0 a)
+| antReturn x a 
+  : annotation (stmtReturn x) (ann0 a)
+| antLet Z s t a sa ta 
+  : annotation s sa 
+    -> annotation t ta 
+    -> annotation (stmtLet Z s t) (ann2 a sa ta).
+
+Instance annotation_dec_inst {A} {s} {a} : Computable (@annotation A s a).
+Proof. 
+  constructor.
+  revert a. induction s; destruct a; try destruct IHs;
+  try (now left; econstructor; eauto);
+  try (now right; inversion 1; eauto).
+  destruct (IHs a0); 
+    try (now left; econstructor; eauto);
+    try (now right; inversion 1; eauto).
+  destruct (IHs1 a2), (IHs2 a3);
+    try (now left; econstructor; eauto);
+    try (now right; inversion 1; eauto).
+  destruct (IHs1 a2), (IHs2 a3);
+    try (now left; econstructor; eauto);
+    try (now right; inversion 1; eauto).
+Defined.
+
+
+(* 
+*** Local Variables: ***
+*** coq-load-path: (("../" "Lvc")) ***
+*** End: ***
+*)
+
