LivenessAnalysis.v
@@ -1,7 +1,7 @@
 Require Import CSet Le.
 
 Require Import Plus Util AllInRel Map CSet.
-Require Import Val Var Env EnvTy IL Lattice DecSolve AbsInt Filter.
+Require Import Val Var Env EnvTy IL Annotation Lattice DecSolve AbsInt Filter.
 
 Instance set_var_semilattice : SemiLattice (set var) := {
   bottom := ∅;
@@ -14,15 +14,15 @@ Defined.
 
 Definition liveness_transform (DL:list (set var * params)) st a :=
   match st, a with
-    | stmtExp x e s as st, annExp d ans => 
+    | stmtExp x e s as st, ann1 d ans => 
       (getAnn ans \ {{x}}) ∪ (if [x ∈ getAnn ans] then Exp.freeVars e else ∅)
-    | stmtIf x s t as st, annIf d ans ant =>
+    | stmtIf x s t as st, ann2 d ans ant =>
       {{x}} ∪ getAnn ans ∪ getAnn ant
-    | stmtGoto f Y as st, annGoto d as an => 
+    | stmtGoto f Y as st, ann0 d as an => 
       let (lv,Z) := nth (counted f) DL (∅,nil) in
       lv \ of_list Z ∪ of_list (filter_by (fun x => B[x ∈ lv]) Z Y)
-    | stmtReturn x as st, annReturn d as an => {{x}}
-    | stmtLet Z s t as st, annLet d ans ant => 
+    | stmtReturn x as st, ann0 d as an => {{x}}
+    | stmtLet Z s t as st, ann2 d ans ant => 
        (getAnn ans \ of_list Z) ∪ getAnn ant
     | _, an => ∅
   end.
